thy/OpenFlow/FeatherweightOpenFlowComparison.thy
@@ -29,7 +29,54 @@ proof -
 	by(rule guha_table_semantics.intros(1)[of \<gamma> ?fe1 p "[]" "[?fe2]", unfolded append_Nil flow_entry_match.sel] | 
 	   rule guha_table_semantics.intros(1)[of \<gamma> ?fe2 p "[?fe1]" "[]", unfolded append_Nil2 flow_entry_match.sel append.simps] |
 	   simp add: m)+
-	thus ?thesis using as by blast
+	thus ?thesis using as by(intro exI conjI)
 qed
+
+lemma guha_umstaendlich: (* or maybe it's Coq where the original formulation is more beneficial *)
+	assumes ae: "a = ofe_action fe"
+	assumes ele: "fe \<in> set ft"
+	assumes rest: "\<gamma> (ofe_fields fe) p" 
+	              "\<forall>fe' \<in> set ft. ofe_prio fe' > ofe_prio fe \<longrightarrow> \<not>\<gamma> (ofe_fields fe') p"
+ 	shows "guha_table_semantics \<gamma> ft p (Some a)"
+proof -
+	from ele obtain ft1 ft2 where ftspl: "ft = ft1 @ fe # ft2" using split_list by fastforce
+	show ?thesis unfolding ae ftspl
+		apply(rule guha_table_semantics.intros(1))
+		using rest(1) apply(simp)
+		using rest(2)[unfolded ftspl] apply simp
+	done
+qed
+
+lemma guha_equal_Action:
+	assumes no: "no_overlaps \<gamma> ft"
+	assumes spm: "OF_same_priority_match3 \<gamma> ft p = Action a"
+	shows "guha_table_semantics \<gamma> ft p (Some a)"
+proof -
+	note spm[THEN OF_spm3_get_fe] then obtain fe where a: "ofe_action fe = a" and fein: "fe \<in> set ft" and feana: "OF_same_priority_match3_ana \<gamma> ft p = Action fe" by blast
+	show ?thesis
+		apply(rule guha_umstaendlich)
+		apply(rule a[symmetric])
+		apply(rule fein)
+		using feana unfolding OF_same_priority_match3_ana_def
+		apply(auto dest!: filter_singleton split: list.splits)
+	done
+qed
+
+lemma guha_equal_NoAction:
+	assumes no: "no_overlaps \<gamma> ft"
+	assumes spm: "OF_same_priority_match3 \<gamma> ft p = NoAction"
+	shows "guha_table_semantics \<gamma> ft p None"
+using spm unfolding OF_same_priority_match3_def
+by(auto simp add: filter_empty_conv OF_spm3_noa_none[OF no spm] intro: guha_table_semantics.intros(2) split: list.splits)
+
+lemma
+	assumes no: "no_overlaps \<gamma> ft"
+	shows "guha_table_semantics \<gamma> ft p (ftb_to_option (OF_same_priority_match3 \<gamma> ft p))"
+unfolding ftb_to_option_def
+	apply(cases "(OF_same_priority_match3 \<gamma> ft p)")
+	apply(simp add: guha_equal_Action[OF no])
+	apply(simp add: guha_equal_NoAction[OF no])
+	apply(subgoal_tac False, simp)
+	using check_no_overlapI no no_overlap_not_unefined no_overlaps_defeq by fastforce
 
 end
